Add low-level cache model

Cpu.fst
@@ -7,33 +7,53 @@ open Value
 type address = FStar.UInt64.t
 type word = FStar.UInt64.t
 
-type systemState
-     = { memory: (memory:memoryState{FStar.UInt.fits (FStar.List.length memory) FStar.UInt64.n});
-             pc: (pc:word{FStar.UInt64.v pc < FStar.List.length memory});
-      registers: memoryState}
+type memory_size = n:int{FStar.UInt.fits n FStar.UInt64.n}
+
+type cache_state (n:memory_size) =
+       (list (a:address{FStar.UInt64.v a < n}))
+
+
+type systemState (#n #r:memory_size)
+     = { memory: (memory:memoryState{(FStar.List.length memory) = n});
+    cache_lines: (list (a:address{FStar.UInt64.v a < n}));
+             pc: (pc:word{FStar.UInt64.v pc < n});
+      registers: (registers:memoryState{FStar.List.length registers = r})}
 
 (* Equivalence *)
-let equiv_system (lhs:systemState) (rhs:systemState)
-    =    (lhs.pc = rhs.pc)
+let equiv_system (#m #q #n #r: memory_size) (lhs:systemState #m #q) (rhs:systemState #n #r)
+    = (m = n)
+       /\ (q = r)
+       /\ (lhs.pc = rhs.pc)
        /\ (equiv_list lhs.registers rhs.registers)
        /\ (equiv_list lhs.memory rhs.memory)
+       /\ (equivalent_lists_have_equal_lengths lhs.memory rhs.memory;
+          lhs.cache_lines = rhs.cache_lines)
 
-let equal_systems_are_equivalent (lhs:systemState) (rhs:systemState):
-  Lemma (requires lhs = rhs) (ensures (equiv_system lhs rhs)) =
+let equal_systems_are_equivalent (#n #r:memory_size) (lhs:systemState #n #r) (rhs:systemState #n #r):
+  Lemma (requires lhs = rhs) (ensures (equiv_system #n #r #n #r lhs rhs)) =
   equal_lists_are_equivalent _ lhs.registers rhs.registers;
   equal_lists_are_equivalent _ lhs.memory rhs.memory
 
-let system_equivalence_is_transitive (lhs mid rhs:systemState):
+let system_equivalence_is_transitive (#m #q #n #r #o #s: memory_size) (lhs:systemState #m #q) (mid:systemState #n #r) (rhs:systemState #o #s):
     Lemma (requires (equiv_system lhs mid) /\ (equiv_system mid rhs))
           (ensures  equiv_system lhs rhs)
     = assert(lhs.pc = rhs.pc);
-      list_equivalence_is_transitive _ lhs.registers mid.registers rhs.registers;
-      list_equivalence_is_transitive _ lhs.memory          mid.memory          rhs.memory
 
-let system_equivalence_is_symmetric (lhs rhs:systemState):
+      list_equivalence_is_transitive _ lhs.registers mid.registers rhs.registers;
+      list_equivalence_is_transitive _ lhs.memory          mid.memory          rhs.memory;
+
+      equivalent_lists_have_equal_lengths lhs.memory rhs.memory;
+      assert(lhs.cache_lines = rhs.cache_lines)
+
+
+let system_equivalence_is_symmetric (#m #q #n #r: memory_size) (lhs: systemState #m #q) (rhs:systemState #n #r):
     Lemma (requires equiv_system lhs rhs)
           (ensures  equiv_system rhs lhs)
     = assert(lhs.pc = rhs.pc);
+
+      equivalent_lists_have_equal_lengths lhs.memory rhs.memory;
+      assert(lhs.cache_lines = rhs.cache_lines);
+
       list_equivalence_is_symmetric _ lhs.registers rhs.registers;
       list_equivalence_is_symmetric _ lhs.memory          rhs.memory
 
@@ -45,24 +65,26 @@ let system_equivalence_is_symmetric (lhs rhs:systemState):
  * blinded values of the system.
  *******************************************************************************)
 
-let redact_system (s:systemState): systemState = {
+let redact_system (#n #r: memory_size) (s:systemState #n #r): systemState #n #r = {
     pc = (redaction_preserves_length _ s.memory 0uL;
           let redacted_memory = redact_list s.memory 0uL in
           s.pc);
+    cache_lines = s.cache_lines;
     registers = (redaction_preserves_length _ s.registers 0uL;
                  redact_list s.registers 0uL);
     memory    = redact_list s.memory 0uL
     }
 
 
-let systems_are_equivalent_to_their_redaction (s:systemState):
+let systems_are_equivalent_to_their_redaction (#n #r: memory_size) (s:systemState #n #r):
     Lemma (ensures equiv_system s (redact_system s))
     = lists_are_equivalent_to_their_redaction  _ s.registers 0uL;
       lists_are_equivalent_to_their_redaction  _ s.memory 0uL
 
-let equivalent_systems_have_equal_redactions (s1:systemState) (s2:systemState):
-    Lemma (ensures (equiv_system s1 s2) <==> ((redact_system s1) == (redact_system s2)))
-    = equivalent_lists_have_equal_redactions _ s1.registers s2.registers 0uL;
+let equivalent_systems_have_equal_redactions (#m #q #n #r: memory_size) (s1:systemState #m #q) (s2:systemState #n #r):
+    Lemma (requires (equiv_system s1 s2)) (ensures ((redact_system s1) == (redact_system s2)))
+    = assert(m = n);
+      equivalent_lists_have_equal_redactions _ s1.registers s2.registers 0uL;
       equivalent_lists_have_equal_redactions _ s1.memory s2.memory 0uL
 
 
@@ -73,12 +95,12 @@ let equivalent_systems_have_equal_redactions (s1:systemState) (s2:systemState):
  * and a function that "steps" the processor state (essentially, the
  * microarchitecture, which for now just fetch-executes in a single step).
  *******************************************************************************)
-type execution_unit = word -> systemState -> systemState
+type execution_unit (#n #r:memory_size) = word -> systemState #n #r -> systemState #n #r
 
-val step
-    (exec:execution_unit)
-    (pre_state: systemState)
-    : systemState
+val step (#n #r:memory_size)
+    (exec:execution_unit #n #r)
+    (pre_state: systemState #n #r)
+    : systemState #n #r
 
 let step exec pre_state =
     let instruction = Memory.nth pre_state.memory pre_state.pc in
@@ -93,13 +115,13 @@ let step exec pre_state =
  * equivalent (and so indistinguishable) states always results in equivalent
  * output states.
  *******************************************************************************)
-let equivalent_inputs_yield_equivalent_states (exec:execution_unit) (pre1 pre2 : systemState) =
+let equivalent_inputs_yield_equivalent_states (#n #r:memory_size) (exec:execution_unit #n #r) (pre1 pre2 : systemState #n #r) =
     equiv_system pre1 pre2 ==> equiv_system (step exec pre1) (step exec pre2)
 
-let is_safe (exec:execution_unit) =
+let is_safe (#n #r:memory_size) (exec:execution_unit #n #r) =
     forall (pre1 pre2 : systemState). equivalent_inputs_yield_equivalent_states exec pre1 pre2
 
-type safe_execution_unit = exec:execution_unit{is_safe exec}
+type safe_execution_unit (#n #r:memory_size) = exec:(execution_unit #n #r){is_safe exec}
 
 (*******************************************************************************
  * Redacting-equivalent execution units.
@@ -109,20 +131,20 @@ type safe_execution_unit = exec:execution_unit{is_safe exec}
  * values zeroed is safe.
  *******************************************************************************)
 
- let is_redacting_equivalent_execution_unit (exec:execution_unit)
+ let is_redacting_equivalent_execution_unit (#n #r:memory_size) (exec:execution_unit #n #r)
    = forall(pre:systemState) (inst:word).  (equiv_system (exec inst pre) (exec inst (redact_system pre)))
 
-type redacting_equivalent_execution_unit
-   = exec:execution_unit{is_redacting_equivalent_execution_unit exec}
+type redacting_equivalent_execution_unit (#n #r:memory_size)
+   = exec:(execution_unit #n #r){is_redacting_equivalent_execution_unit exec}
 
-let is_redacting_equivalent_system_single_step_somewhere (exec:execution_unit) (pre:systemState) =
+let is_redacting_equivalent_system_single_step_somewhere (#n #r:memory_size) (exec:execution_unit #n #r) (pre:systemState #n #r) =
     (equiv_system (step exec pre) (step exec (redact_system pre)))
 
-let is_redacting_equivalent_system_single_step_everywhere (exec:execution_unit) =
+let is_redacting_equivalent_system_single_step_everywhere (#n #r:memory_size) (exec:execution_unit #n #r) =
     forall (pre:systemState). is_redacting_equivalent_system_single_step_somewhere exec pre
 
-let redacting_equivalent_execution_units_lead_to_redacting_equivalent_systems_somewhere
-    (exec:redacting_equivalent_execution_unit) (pre:systemState):
+let redacting_equivalent_execution_units_lead_to_redacting_equivalent_systems_somewhere (#n #r:memory_size)
+    (exec:redacting_equivalent_execution_unit #n #r) (pre:systemState #n #r):
     Lemma (ensures is_redacting_equivalent_system_single_step_somewhere exec pre) =
       let redaction = redact_system pre in
       systems_are_equivalent_to_their_redaction pre;
@@ -132,8 +154,8 @@ let redacting_equivalent_execution_units_lead_to_redacting_equivalent_systems_so
       assert(equiv_list pre.memory redaction.memory);
       assert(equiv (Memory.nth pre.memory pc) (Memory.nth redaction.memory pc))
 
-let redacting_equivalent_systems_give_equivalent_outputs_for_equivalent_inputs
-    (exec:redacting_equivalent_execution_unit) (pre_1:systemState) (pre_2:systemState)
+let redacting_equivalent_systems_give_equivalent_outputs_for_equivalent_inputs (#n #r:memory_size)
+    (exec:redacting_equivalent_execution_unit #n #r) (pre_1:systemState #n #r) (pre_2:systemState #n #r)
       : Lemma (requires equiv_system pre_1 pre_2)
               (ensures equiv_system (step exec pre_1) (step exec pre_2))
               [SMTPat (equiv_system (step exec pre_1) (step exec pre_2))]
@@ -146,8 +168,8 @@ let redacting_equivalent_systems_give_equivalent_outputs_for_equivalent_inputs
         system_equivalence_is_transitive (step exec pre_1) (step exec (redact_system pre_1)) (step exec pre_2)
 
 (* The main theorem about execution_units *)
-let redacting_equivalent_execution_units_are_safe
-    (exec:redacting_equivalent_execution_unit):
+let redacting_equivalent_execution_units_are_safe (#n #r:memory_size)
+    (exec:redacting_equivalent_execution_unit #n #r):
     Lemma (ensures is_safe exec)
       = ()
 
